Condensed all binary operators into a single constructor with a SymOp field to reduce the number of SymExpr constructors.

compcert-1.8/ia32/Peephole.v
@@ -37,8 +37,31 @@ Inductive Loc : Type :=
   | Register : preg -> Loc
   | Memory   : addrmode -> Loc.
 
+Inductive SymOp :=
+  | SymAdd
+  | SymSub
+  | SymMult
+  | SymDivU
+  | SymDivS
+  | SymModU
+  | SymModS
+  | SymShiftR
+  | SymShiftRU
+  | SymROR
+  | SymAnd
+  | SymOr
+  | SymXor
+  | SymCmp
+  | SymTest
+  | SymAddF
+  | SymSubF
+  | SymMultF
+  | SymDivF.
+
 Inductive SymExpr : Type :=
   (* Integers *)
+  | binOp  : SymOp   -> SymExpr -> SymExpr -> SymExpr
+(*
   | add    : SymExpr -> SymExpr -> SymExpr
   | sub    : SymExpr -> SymExpr -> SymExpr
   | mult   : SymExpr -> SymExpr -> SymExpr
@@ -51,9 +74,14 @@ Inductive SymExpr : Type :=
   | ror    : SymExpr -> SymExpr -> SymExpr
   | and    : SymExpr -> SymExpr -> SymExpr
   | or     : SymExpr -> SymExpr -> SymExpr
-  | neg    : SymExpr -> SymExpr
   | xor    : SymExpr -> SymExpr -> SymExpr
+
+
+*)
+  | neg    : SymExpr -> SymExpr
+
   (* Tests *)
+(*
   | cmp    : SymExpr -> SymExpr -> SymExpr
   | test   : SymExpr -> SymExpr -> SymExpr  (* modifies x86 status register! *) 
   (* Floating *)
@@ -61,10 +89,31 @@ Inductive SymExpr : Type :=
   | sub_f  : SymExpr -> SymExpr -> SymExpr
   | mult_f : SymExpr -> SymExpr -> SymExpr
   | div_f  : SymExpr -> SymExpr -> SymExpr
+  *)
   | abs_f  : SymExpr -> SymExpr
   | neg_f  : SymExpr -> SymExpr
   | Imm    : val -> SymExpr
   | Initial : Loc -> SymExpr.
+
+Definition cmp := binOp SymCmp.
+Definition test := binOp SymTest.
+Definition add := binOp SymAdd.
+Definition sub := binOp SymSub.
+Definition mult := binOp SymMult.
+Definition div_unsigned := binOp SymDivU.
+Definition div_signed := binOp SymDivS.
+Definition mod_unsigned := binOp SymModU.
+Definition mod_signed := binOp SymModS.
+Definition shiftR := binOp SymShiftR.
+Definition shiftR_unsigned := binOp SymShiftRU.
+Definition ror := binOp SymROR.
+Definition and := binOp SymAnd.
+Definition or := binOp SymOr.
+Definition xor := binOp SymXor.
+Definition add_f := binOp SymAddF.
+Definition sub_f := binOp SymSubF.
+Definition mult_f := binOp SymMultF.
+Definition div_f := binOp SymDivF.
 
 (* here we use a map to store SymExpr in the symbolic execution. This
 may not be the right choice because it's not immediately apparent how
@@ -77,6 +126,19 @@ Proof.
   decide equality. 
   apply preg_eq.
   repeat decide equality; try apply Int.eq_dec.
+Defined.
+
+Lemma SymOp_eq : forall (x y : SymOp), {x = y} + {x <> y}.
+Proof.
+  decide equality.
+Defined.
+
+Definition SymExpr_dec : forall (a b : SymExpr), {a = b} + {a <> b}.
+  refine (fix f (a b : SymExpr) : {a = b} + {a <> b} :=
+    match a, b as _ return _ with
+      | binOp _ _ _, _ => _
+      | _,_ => _
+    end); decide equality; try (apply val_eq_dec); try (apply Loc_eq) ; try (apply SymOp_eq).
 Defined.
 
 (* the type of our location store *)
@@ -402,48 +464,6 @@ Notation "a '&&&' b" :=
     else Utils.in_right).
 
 
-Definition SymExpr_dec : forall (a b : SymExpr), {a = b} + {a <> b}.
-  refine (fix f (a b : SymExpr) : {a = b} + {a <> b} :=
-    match a, b as _ return _ with
-      | add _ _, _ => _
-      | _,_ => _
-    end); decide equality; try (apply val_eq_dec); try (apply Loc_eq). 
-Defined.
-
-
-(* don't actually try to run this definition, it's *very* big and *very* slow... *)
-Definition SymExpr_dec : forall (a b : SymExpr), {a = b} + {a <> b}.
-  refine (fix f (a b : SymExpr) : {a = b} + {a <> b} :=
-  (match a, b as _ return _ with
-     | add _ _, add _ _ => Utils.in_left
-     | sub _ _, sub _ _ => Utils.in_left
-     | mult _ _, mult _ _ => Utils.in_left
-     | div_unsigned _ _, div_unsigned _ _ => Utils.in_left 
-     | div_signed _ _, div_signed _ _ => Utils.in_left
-     | mod_unsigned _ _, mod_unsigned _ _ => Utils.in_left
-     | mod_signed _ _, mod_signed _ _ => Utils.in_left
-     | shiftR _ _, shiftR _ _ => Utils.in_left
-     | shiftR_unsigned _ _, shiftR_unsigned _ _ => Utils.in_left
-     | ror _ _, ror _ _ => Utils.in_left
-     | and _ _, and _ _ => Utils.in_left
-     | or _ _, or _ _ => Utils.in_left
-     | neg _, neg _ => Utils.in_left
-     | xor _ _, xor _ _ => Utils.in_left
-     | cmp _ _, cmp _ _ => Utils.in_left
-     | test _ _, test _ _ =>  Utils.in_left
-     | add_f _ _, add_f _ _ => Utils.in_left
-     | sub_f _ _, sub_f _ _ => Utils.in_left
-     | mult_f _ _, mult_f _ _ => Utils.in_left
-     | div_f _ _, div_f _ _ => Utils.in_left
-     | abs_f _, abs_f _ => Utils.in_left
-     | neg_f _, neg_f _ => Utils.in_left
-
-     | Imm a' , Imm b' => if val_eq_dec a' b' then Utils.in_left else Utils.in_right
-     | Initial a', Initial b' => if Loc_eq a' b' then Utils.in_left else Utils.in_right
-     | _, _ => Utils.in_right
-  end)).   Admitted. (*try decide equality; try (apply Loc_eq); try (apply val_eq_dec). 
-Defined.*)
-
 Fixpoint allLocs_dec (l : list Loc) (a b : locs) : bool :=
   match l with
     | nil => true
@@ -506,13 +526,6 @@ Proof.
   destruct ssE. assumption. simpl. apply leb_n_n_true. simpl. apply leb_n_n_true.
 Qed.
 
-Lemma eq_length_eq : forall A (xs : list A) ys, xs = ys -> length xs = length ys.
-Proof.
-  intros.
-  induction xs. destruct ys ; auto. inversion H.
-  destruct ys. inversion H. rewrite H.  reflexivity.
-Qed.
-
 Fixpoint partitionSymExec (c : Asm.code) : (Asm.code * Asm.code) :=
   match c with
     | nil     => (pair nil nil)
@@ -529,7 +542,7 @@ Function optimize (c : Asm.code) {measure length c} : Asm.code :=
                  | (r::rs) => opt_window (fst part) ++ (r :: optimize rs)
     end.
 Proof.
-  intros.  
+  intros.
 Admitted.
 
 Definition transf_function (f: Asm.code) : res Asm.code :=
